aarch64 refine+crefine: GIC_v3 proof updates
- abstract over the value of max_armKSGICVCPUNumListRegs
- adjust virq access proofs
- abstract over vcpu type size in C (changes with GIC version, because
  number of LR registers changes)

Signed-off-by: Gerwin Klein <gerwin.klein@proofcraft.systems>

proof/refine/AARCH64/ArchInvsDefs_H.thy
@@ -216,7 +216,7 @@ definition valid_asid_table' :: "(asid \<rightharpoonup> machine_word) \<Rightar
 definition "is_vcpu' \<equiv> \<lambda>ko. \<exists>vcpu. ko = (KOArch (KOVCPU vcpu))"
 
 definition max_armKSGICVCPUNumListRegs :: nat where
-  "max_armKSGICVCPUNumListRegs \<equiv> 63"
+  "max_armKSGICVCPUNumListRegs \<equiv> if config_ARM_GIC_V3 then 16 else 64"
 
 definition valid_arch_state' :: "kernel_state \<Rightarrow> bool" where
   "valid_arch_state' \<equiv> \<lambda>s.
